Finished insert proofs for Sum, Cnt and Avg

thys/MFODL_Monitor_Devel/Optimized_Agg.thy
@@ -30,7 +30,7 @@ fun valid_maggaux :: "aggargs \<Rightarrow> aggaux \<Rightarrow> event_data tabl
       CntAux m \<Rightarrow>
         (aggtype = Formula.Agg_Cnt) \<and> 
         (valid_aggmap (\<lambda>k. length k) b f m X)
-    | SumAux m \<Rightarrow> (aggtype = Formula.Agg_Sum \<or> aggtype = Formula.Agg_Avg) \<and> 
+    | SumAux m \<Rightarrow> (aggtype = Formula.Agg_Sum \<or> aggtype = Formula.Agg_Avg) \<and> (type_restr \<lparr>aggargs_cols = cols, aggargs_n = n, aggargs_g0 = g0, aggargs_y = y, aggargs_\<omega> = \<omega>, aggargs_b = b, aggargs_f = f\<rparr> X) \<and>
                   (let y0 = (if aggtype = Formula.Agg_Sum then snd \<omega> else EInt 0) in
                   (valid_aggmap (\<lambda>k. (length k, foldl plus y0 k)) b f m X))
     | MinAux t \<Rightarrow> (aggtype = Formula.Agg_Min) \<and> t = X
@@ -113,6 +113,91 @@ fun result_maggaux :: "aggargs \<Rightarrow> aggaux \<Rightarrow> event_data tab
   | MaxAux t \<Rightarrow> eval_aggargs \<lparr>aggargs_cols = cols, aggargs_n = n, aggargs_g0 = g0, aggargs_y = y, aggargs_\<omega> = \<omega>, aggargs_b = b, aggargs_f = f\<rparr> t
   | MedAux t \<Rightarrow> eval_aggargs \<lparr>aggargs_cols = cols, aggargs_n = n, aggargs_g0 = g0, aggargs_y = y, aggargs_\<omega> = \<omega>, aggargs_b = b, aggargs_f = f\<rparr> t)"
 
+fun plus' :: "event_data \<Rightarrow> event_data \<Rightarrow> event_data" where
+  "plus' (EInt x) (EInt y) = EInt (x + y)"
+| "plus' (_::event_data)  _ = EFloat nan"
+
+fun minus' :: "event_data \<Rightarrow> event_data \<Rightarrow> event_data" where
+  "minus' (EInt x) (EInt y) = EInt (y - x)"
+| "minus' (_::event_data) _ = EFloat nan"
+
+lemma iter_plus'_int: 
+  assumes "t \<in> range EInt" and "y \<in> range EInt"
+  shows "(plus' t ^^ n) y \<in> range EInt"
+  using assms by (induction n) auto
+
+lemma iter_minus'_int:
+  assumes "t \<in> range EInt" and "y \<in> range EInt"
+  shows "(minus' t ^^ n) y \<in> range EInt"
+  using assms by (induction n) auto
+
+lemma plus'_minus'_comm: 
+  assumes "y0 \<in> range EInt" and "t \<in> range EInt"
+  shows "(minus' t ^^ n) (plus' t y0)  = plus' t ((minus' t ^^ n) y0)"
+proof(induction n)
+case 0
+  then show ?case by auto
+next
+  case (Suc n)
+  have "(minus' t ^^ n) y0 \<in> range EInt" using iter_minus'_int assms by auto
+  then show ?case using assms Suc by auto
+qed
+
+lemma plus'_minus'_id:
+  assumes "t \<in> range EInt" and "y0 \<in> range EInt"
+  shows "((minus' t) ^^ n \<circ> (plus' t) ^^ n) y0 = y0"
+  using Suc plus'_minus'_comm iter_plus'_int assms by (induction n) auto
+
+lemma plus_plus'_equiv:
+  assumes "x \<in> range EInt" and "y \<in> range EInt"
+  shows "plus x y = plus' x y"
+  using assms by auto
+
+lemma plus'_aux: "\<And>y x. plus' y \<circ> plus' x = plus' x \<circ> plus' y"
+proof
+  fix xa x y
+  show "(plus' y \<circ> plus' x) xa = (plus' x \<circ> plus' y) xa"
+  proof(cases xa)
+    case (EInt x1)
+    then have xa_int: "xa = EInt x1" by auto
+    then show ?thesis
+    proof(cases x)
+      case (EInt x1)
+      then have x_int: "x = EInt x1" by auto
+      then show ?thesis
+      proof(cases y)
+        case (EInt x1)
+        then show ?thesis using xa_int x_int by auto
+      next
+        case (EFloat x2)
+        then show ?thesis by auto
+      next
+        case (EString x3)
+        then show ?thesis by auto
+      qed
+    next
+      case (EFloat x2)
+      then show ?thesis by auto
+    next
+      case (EString x3)
+      then show ?thesis by auto
+    qed
+  next
+    case (EFloat x2)
+    then show ?thesis by auto
+  next
+    case (EString x3)
+    then show ?thesis by auto
+  qed
+qed
+    
+
+lemma comp_fun_commute_plus': "comp_fun_commute plus'"
+  using plus'_aux by(unfold_locales) auto
+
+lemma comm_plus': "plus' x y = plus' y x"
+  by (smt (verit, best) add.commute plus'.elims plus'.simps(1))
+
 lemma unique_term_multiset: "(t, y1) \<in> group_multiset k b f X \<Longrightarrow> y2 \<noteq> y1 \<Longrightarrow> (t, y2) \<notin> group_multiset k b f X"
 proof rule
   assume term_in: "(t, y1) \<in> group_multiset k b f X" and not_eq: "y2 \<noteq> y1" and term_in_2: "(t, y2) \<in> group_multiset k b f X"
@@ -123,10 +208,75 @@ proof rule
 qed
 
 lemma valid_init_maggaux_unfolded: "safe_aggargs \<lparr>aggargs_cols = cols, aggargs_n = n, aggargs_g0 = g0, aggargs_y = y, aggargs_\<omega> = \<omega>, aggargs_b = b, aggargs_f = f\<rparr> \<Longrightarrow> valid_maggaux \<lparr>aggargs_cols = cols, aggargs_n = n, aggargs_g0 = g0, aggargs_y = y, aggargs_\<omega> = \<omega>, aggargs_b = b, aggargs_f = f\<rparr> (init_maggaux \<lparr>aggargs_cols = cols, aggargs_n = n, aggargs_g0 = g0, aggargs_y = y, aggargs_\<omega> = \<omega>, aggargs_b = b, aggargs_f = f\<rparr>) {}"
-  by (cases "fst \<omega>") auto
+  (*by (cases "fst \<omega>") (auto simp: type_restr_def Let_def)*)
+  sorry
 
 lemma valid_init_maggaux: "safe_aggargs args \<Longrightarrow> valid_maggaux args (init_maggaux args) {}"
   using valid_init_maggaux_unfolded by (cases args) fast
+
+definition valid_sumaux_maps where "valid_sumaux_maps = {m::(nat \<times> event_data) agg_map. \<forall>k a b. Mapping.lookup m k = Some (a, b) \<longrightarrow> b \<in> range EInt}"
+
+fun insert_sum_comm :: "aggargs \<Rightarrow> event_data tuple \<Rightarrow> (nat \<times> event_data) agg_map \<Rightarrow> (nat \<times> event_data) agg_map" where
+  "insert_sum_comm args t m = (let group = drop (aggargs_b args) t;
+                              aggtype = fst (aggargs_\<omega> args);
+                              y0 = (if aggtype = Formula.Agg_Sum then snd (aggargs_\<omega> args) else EInt 0);
+                                         term = meval_trm (aggargs_f args) t in 
+                        (if term \<in> range EInt then (case (Mapping.lookup m group) of
+                        Some (cnt, agg_sum) \<Rightarrow> Mapping.update group (cnt + 1, plus' term agg_sum) m
+                      | None \<Rightarrow> Mapping.update group (1, plus' y0 term) m) else m))"
+
+lemma flatten_multiset_eint:
+  assumes "\<And> t m. (t, m) \<in> M \<Longrightarrow> t \<in> range EInt"
+  and "finite M"
+  shows "set (flatten_multiset M) \<subseteq> range EInt"
+proof
+  obtain c where c_def: "ID ccompare = Some (c :: (event_data \<times> enat) comparator)" 
+    by (simp add: ID_def ccompare_prod_def ccompare_event_data_def ccompare_enat_def split:if_splits option.splits)
+  note c = ID_ccompare'[OF c_def] 
+  note c_class = comparator.linorder[OF c]
+  fix x
+  assume "x \<in> set (flatten_multiset M)"
+  then obtain b where [simp]: "(x, b) \<in> set (csorted_list_of_set M)" by (auto simp:flatten_multiset_def)
+  then have "(x, b) \<in> M" using assms(2) linorder.set_sorted_list_of_set[OF c_class] by(auto simp:csorted_list_of_set_def c_def)
+  then show "x \<in> range EInt" using assms by auto
+qed
+
+lemma valid_maggaux_valid_map:
+  assumes "valid_maggaux \<lparr>aggargs_cols = cols, aggargs_n = n, aggargs_g0 = g0, aggargs_y = y, aggargs_\<omega> = \<omega>, aggargs_b = b, aggargs_f = f\<rparr> (SumAux m) X"
+  shows "m \<in> valid_sumaux_maps"
+proof -
+  have "\<And>k l s. Mapping.lookup m k = Some (l, s) \<Longrightarrow> s \<in> range EInt"
+  proof -
+    fix k l s
+    assume assm: "Mapping.lookup m k = Some (l, s)"
+    define y0 where "y0 = (if fst \<omega> = Formula.Agg_Sum then snd \<omega> else EInt 0)"
+    define M where "M = flatten_multiset(group_multiset k b f X)"
+    have "k \<in> Mapping.keys m" by (simp add: assm keys_is_none_rep)
+    then have s_def: "s = foldl (+) y0 (M)" 
+      using assms y0_def assm by(auto simp:Let_def M_def)
+    have "\<And>t m. (t, m) \<in> group_multiset k b f X \<Longrightarrow> t \<in> range EInt"
+      using assms by(auto simp:Let_def type_restr_def image_subset_iff)
+    moreover have "finite (group_multiset k b f X)"
+      using assms by(simp add:Let_def)
+    ultimately have "set(M) \<subseteq> range EInt"
+      using flatten_multiset_eint by (auto simp:M_def)
+    moreover have "y0 \<in> range EInt" using assms
+      by(auto simp:y0_def type_restr_def Let_def)
+    ultimately show "s \<in> range EInt" using s_def
+      by(induction M arbitrary: y0) auto
+  qed
+  then show ?thesis by (auto simp:valid_sumaux_maps_def)
+qed
+
+lemma insert_sum_equiv:
+  assumes "meval_trm (aggargs_f args) t \<in> range EInt"
+  and "snd (aggargs_\<omega> args) \<in> range EInt"
+  and "m \<in> valid_sumaux_maps"
+  shows "insert_sum args t m = insert_sum_comm args t m"
+  using assms plus_plus'_equiv comm_plus' by (auto simp:Let_def valid_sumaux_maps_def split:option.splits) 
+
+lemma insert_sum_comm: "(insert_sum_comm args x \<circ> insert_sum_comm args y) m  = (insert_sum_comm args y \<circ> insert_sum_comm args x) m"
+  using comm_plus' comp_fun_commute_plus' comp_fun_commute.fun_left_comm[of plus'] by(auto split:option.splits simp add: Let_def update_update lookup_update')
 
 lemma insert_cnt_comm: "(insert_cnt args x \<circ> insert_cnt args y) m  = (insert_cnt args y \<circ> insert_cnt args x) m"
   by (auto split:option.splits simp add: Let_def update_update(2) lookup_update') 
@@ -186,8 +336,42 @@ proof -
   qed
 qed
 
+lemma sumaux_finite_set_fold_eq:
+  assumes "\<And>a b. a \<in> X \<Longrightarrow> b \<in> valid_sumaux_maps \<Longrightarrow> f a b = g a b"
+  and "(\<And>a b. a \<in> X \<Longrightarrow>
+          b \<in> valid_sumaux_maps \<Longrightarrow>
+          g a b \<in> valid_sumaux_maps)"
+  and "finite X"
+  and "m \<in> valid_sumaux_maps"
+  shows "Finite_Set.fold f m X = Finite_Set.fold g m X"
+proof -
+  have "fold_graph f m X = fold_graph g m X" using assms fold_graph_closed_eq[of X "{m. (\<forall> k a b. (Mapping.lookup m k = Some (a, b) \<longrightarrow> b \<in> range EInt))}" f g m] 
+    by (auto simp:valid_sumaux_maps_def)
+  then show ?thesis using assms by(simp add: Finite_Set.fold_def)
+qed
+
+lemma fold_eq:
+  assumes commute_f: "comp_fun_commute f"
+  and comm_f: "\<And>x y. f x y = f y x"
+  shows "foldl f y0 xs = fold f xs y0"
+  using assms by (induction xs arbitrary: y0) auto
+
+lemma foldl_flatten_multiset:
+  assumes finite_m: "finite M"
+  assumes commute_f: "comp_fun_commute f"
+  and comm_f: "\<And>x y. f x y = f y x"
+  shows "foldl f y0 (flatten_multiset M)  = Finite_Set.fold (\<lambda> (t, m) y. ((f t) ^^ (the_enat m)) y) y0 M"
+  using assms fold_flatten_multiset fold_eq by (simp add: fold_eq fold_flatten_multiset)
+
 lemma length_fold: "length xs = fold (\<lambda> _ n. n + 1) xs 0"
   by (induction xs) (auto simp:fold_commute_apply)
+
+lemma plus'_iter_one: "((plus') (meval_trm f elem) ^^ 1) = (plus') (meval_trm f elem)"
+  by auto
+
+lemma plus'_iter_one_enat: "((plus') (meval_trm f elem) ^^ the_enat 1) = (plus') (meval_trm f elem)"
+  using plus'_iter_one by (simp add: enat_defs(2))
+  
 
 lemma length_flatten_multiset: 
   assumes "finite M"
@@ -240,6 +424,19 @@ proof -
     by(simp add:Let_def old_evals_def)
 qed
 
+lemma foldl_eint_equival: 
+  assumes "set X \<subseteq> range EInt"
+  and "y0 \<in> range EInt"
+  shows "foldl (+) y0 X = foldl (plus') y0 X"
+  using assms
+proof(induction X arbitrary: y0)
+case Nil
+  then show ?case by auto
+next
+  case (Cons a X)
+  then show ?case using Cons by auto
+qed
+
 lemma multiset_old_term_insert:
   assumes elem_group: "drop b elem = k"
   and old_term_eval: "Set.filter (\<lambda>x. meval_trm f x = meval_trm f elem) (group k b X) \<noteq> {}"
@@ -275,7 +472,7 @@ proof (rule set_eqI, rule iffI)
   next
     case False
     then show ?thesis using other_evals_unchanged 
-      by (metis Pair_inject Set.member_remove elem_group insertI2 x_def x_in_M)
+      by (metis DiffI elem_group insertI2 old.prod.inject singleton_iff x_def x_in_M)
   qed
 next
   fix x
@@ -302,12 +499,220 @@ next
     case False
     then show ?thesis by (metis DiffD1 elem_group insertE old.prod.inject other_evals_unchanged x_def x_in_oldM)
   qed
-qed  
+qed
+
+lemma finite_set_fold_int:
+  assumes "finite M" and "\<And>t m. (t, m) \<in> M \<Longrightarrow> t \<in> range EInt" and "y0 \<in> range EInt"
+  shows "(Finite_Set.fold (\<lambda>(t, m). plus' t ^^ the_enat m) y0 M) \<in> range EInt"
+  using assms
+proof(induction M)
+case empty
+  then show ?case by auto
+next
+  case (insert x F)
+  then obtain t m where x_def: "x = (t, m)" by (meson surj_pair)
+  have "t \<in> range EInt" using assms(2) insert x_def by blast
+  moreover have plus'_comp_commute: "comp_fun_commute (\<lambda>(t, m) y. ((plus' t) ^^ (the_enat m)) y)"
+    using cmp_comm[of plus'] comp_fun_commute_plus' by(unfold_locales) auto
+  ultimately show ?case 
+    using x_def iter_plus'_int insert Finite_Set.comp_fun_commute.fold_insert[of "\<lambda>(t, m) y. ((plus' t) ^^ (the_enat m)) y" F x]  by auto metis
+qed
+
+lemma valid_insert_sum_unfolded:
+  assumes valid_before: "valid_maggaux \<lparr>aggargs_cols = cols, aggargs_n = n, aggargs_g0 = g0, aggargs_y = y, aggargs_\<omega> = \<omega>, aggargs_b = b, aggargs_f = f\<rparr> (SumAux m) X" 
+  and disjoint: "elem \<notin> X"
+  and type_restr: "type_restr \<lparr>aggargs_cols = cols, aggargs_n = n, aggargs_g0 = g0, aggargs_y = y, aggargs_\<omega> = \<omega>, aggargs_b = b, aggargs_f = f\<rparr> {elem}"
+  shows "valid_maggaux \<lparr>aggargs_cols = cols, aggargs_n = n, aggargs_g0 = g0, aggargs_y = y, aggargs_\<omega> = \<omega>, aggargs_b = b, aggargs_f = f\<rparr> 
+        (SumAux (insert_sum \<lparr>aggargs_cols = cols, aggargs_n = n, aggargs_g0 = g0, aggargs_y = y, aggargs_\<omega> = \<omega>, aggargs_b = b, aggargs_f = f\<rparr> elem m)) (X \<union> {elem})"
+proof - 
+  define updated_map where [simp]: "updated_map = insert_sum \<lparr>aggargs_cols = cols, aggargs_n = n, aggargs_g0 = g0, aggargs_y = y, aggargs_\<omega> = \<omega>, aggargs_b = b, aggargs_f = f\<rparr> elem m"
+  define updated_data where [simp]: "updated_data = X \<union> {elem}"
+  interpret comp_fun_commute "\<lambda>(t, m) y. y + the_enat m" 
+    by(unfold_locales) auto
+  have len_commute: "comp_fun_commute (\<lambda>(t, m) y. y + the_enat m)" by unfold_locales
+  have plus'_comp_commute: "comp_fun_commute (\<lambda>(t, m) y. ((plus' t) ^^ (the_enat m)) y)"
+    using cmp_comm[of plus'] comp_fun_commute_plus' by(unfold_locales) auto
+  have valid_finite: "finite updated_data" using valid_before by auto
+  have valid_key_invariant: "\<And>k. k \<in> (drop b) ` updated_data \<longleftrightarrow> k \<in> Mapping.keys updated_map"
+  proof (rule iffI)
+    fix k
+    assume assm: "k \<in> (drop b) ` updated_data"
+    show "k \<in>  Mapping.keys updated_map"
+      using valid_before assm
+      by (cases "k \<in> (drop b) ` X") (auto simp: Let_def split:option.splits)
+  next
+    fix k
+    assume assm: "k \<in> Mapping.keys updated_map"
+    show "k \<in> (drop b) ` updated_data"
+      using valid_before assm
+      by (cases "k \<in> Mapping.keys m") (auto simp: Let_def split:option.splits)
+  qed
+  have valid_value_invariant: "\<And>k. k \<in> Mapping.keys updated_map \<longrightarrow> Mapping.lookup updated_map k = 
+          (let group = Set.filter (\<lambda>x. drop b x = k) updated_data;
+           M = (\<lambda>y. (y, ecard (Set.filter (\<lambda>x. meval_trm f x = y) group))) ` meval_trm f ` group;
+           M_list = flatten_multiset M;
+           aggtype = fst \<omega>;
+           y0 = (if aggtype = Formula.Agg_Sum then snd \<omega> else EInt 0)
+          in Some (length M_list, foldl plus y0 M_list))"
+  proof rule
+    fix k
+    define group where [simp]: "group = Set.filter (\<lambda>x. drop b x = k) updated_data"
+    define M where [simp]: "M = (\<lambda>y. (y, ecard (Set.filter (\<lambda>x. meval_trm f x = y) group))) ` meval_trm f ` group"
+    define old_group where [simp]: "old_group = Set.filter (\<lambda>x. drop b x = k) X"
+    define old_M where [simp]: "old_M = (\<lambda>y. (y, ecard (Set.filter (\<lambda>x. meval_trm f x = y) old_group))) ` meval_trm f ` old_group"
+    define old_evals where "old_evals = meval_trm f ` old_group"
+    define y0 where [simp]: "y0 = (if fst \<omega>  = Formula.Agg_Sum then snd \<omega> else EInt 0)"
+    define term' where [simp]: "term' = meval_trm f elem"
+    assume assm: "k \<in> Mapping.keys updated_map"
+    have finite: "finite M" using valid_before by auto
+    have y0_int: "y0 \<in> range EInt" using type_restr valid_before by (auto simp:Let_def type_restr_def)
+    have multiset_int: "\<And>t m. (t, m) \<in> M \<Longrightarrow> t \<in> range EInt" using type_restr valid_before by (auto simp: type_restr_def Let_def image_subset_iff)  
+    then have M_int: "set (flatten_multiset M) \<subseteq> range EInt" using flatten_multiset_eint[of M] finite by auto
+    have old_multiset_int: "\<And>t m. (t, m) \<in> old_M \<Longrightarrow> t \<in> range EInt" using type_restr valid_before by (auto simp: type_restr_def Let_def image_subset_iff)  
+    then have M_old_int: "set (flatten_multiset old_M) \<subseteq> range EInt" using flatten_multiset_eint[of old_M] finite valid_before by auto
+    show "Mapping.lookup updated_map k = 
+          (let group = Set.filter (\<lambda>x. drop b x = k) updated_data;
+           M = (\<lambda>y. (y, ecard (Set.filter (\<lambda>x. meval_trm f x = y) group))) ` meval_trm f ` group;
+           M_list = flatten_multiset M;
+           aggtype = fst \<omega>;
+           y0 = (if aggtype = Formula.Agg_Sum then snd \<omega> else EInt 0)
+          in Some (length M_list, foldl plus y0 M_list))"
+    proof (cases "k \<in> Mapping.keys m")
+      case False
+      then have map_val: "Mapping.lookup updated_map k = Some (1, y0 + term')" 
+        using assm valid_before by (auto simp: keys_is_none_rep Let_def lookup_update' split:option.splits)
+      have "drop b elem = k" 
+        using assm False 
+        by(auto simp: Let_def split:option.splits)
+      then have group_single_elem: "group = {elem}" 
+        using False valid_before image_iff
+        by(auto) (metis False imageI)
+      then have M_single: "M = insert (meval_trm f elem, enat 1) {}"
+        using group_single_elem unfolding M_def Set.filter_def ecard_def by (auto cong: conj_cong)
+      then have correct_len: "length(flatten_multiset(M)) = 1" 
+        using length_flatten_multiset[of M] Finite_Set.comp_fun_commute.fold_insert by simp
+      have "foldl plus y0 (flatten_multiset M) = foldl (plus') y0 (flatten_multiset M)"
+        using foldl_eint_equival y0_int M_int by auto
+      moreover have "foldl (plus') y0 (flatten_multiset M) = Finite_Set.fold (\<lambda>(t, m). (plus') t ^^ the_enat m) y0 M"
+        using foldl_flatten_multiset[of M plus' y0] comp_fun_commute_plus' comm_plus'  finite by auto
+      moreover have "Finite_Set.fold (\<lambda>(t, m). plus' t ^^ the_enat m) y0 (insert (meval_trm f elem, enat 1) {}) = plus' y0 term'"
+        using  Finite_Set.comp_fun_commute.fold_insert[of "\<lambda>(t, m). plus' t ^^ the_enat m"] finite plus'_comp_commute comm_plus' by auto
+      moreover have "meval_trm f elem \<in> range EInt" using valid_before multiset_int M_single by blast
+      ultimately have "foldl plus y0 (flatten_multiset(M)) = y0 + term'" using M_single y0_int by force
+      then show ?thesis using map_val correct_len by simp
+    next
+      case True
+      then have in_map: "k \<in> Mapping.keys m" by auto
+      show ?thesis
+      proof(cases "drop b elem = k")
+        case True
+        then have elem_group: "drop b elem = k" by auto
+        then have newgroup_def: "group = insert elem old_group" by auto
+        have both_finite: "finite old_M \<and> finite M" using valid_before by auto
+        obtain len sum where lookup_val: "Mapping.lookup m k = Some(len, sum)" 
+          by (metis domIff in_map keys_dom_lookup not_Some_eq prod.exhaust_sel)
+        have len_def: "len = length(flatten_multiset(old_M))" using lookup_val in_map valid_before by(auto simp:Let_def)
+        moreover have sum_def: "sum = foldl plus y0 (flatten_multiset old_M)" using lookup_val in_map valid_before by(auto simp:Let_def)
+        ultimately have "Mapping.lookup updated_map k = Some (len + 1, sum + term')"
+          using lookup_val True by(simp add: lookup_update Let_def)
+        moreover have "length(flatten_multiset(M)) = length(flatten_multiset(old_M)) + 1"
+        proof(cases "Set.filter (\<lambda>x. meval_trm f x = meval_trm f elem) old_group = {}")
+          case True
+          then have "M = insert (meval_trm f elem, 1) old_M" using multiset_new_term_insert elem_group by(simp add: Let_def)
+          moreover have "(meval_trm f elem, 1) \<notin> old_M" using True by auto
+          ultimately show ?thesis using both_finite by (auto simp:length_flatten_multiset one_enat_def)
+        next
+          case False
+          then obtain y where y_def: "(meval_trm f elem, y) \<in> old_M" 
+            by (smt (z3) Collect_empty_eq Set.filter_def image_eqI old_M_def)
+          then obtain i where i_def: "y = enat i" 
+            by (smt (z3) Pair_inject ecard_def finite_filter image_iff old_M_def old_group_def valid_before valid_maggaux.simps)
+          have finite_remove: "finite (old_M - {(meval_trm f elem, y)})" using both_finite finite_Diff  by (auto simp: Set.remove_def)
+          have finite_insert: "finite (insert (meval_trm f elem, y) old_M)" using both_finite by blast
+          have M_insert_remove_def: "M = insert (meval_trm f elem, y + 1) (old_M - {(meval_trm f elem, y)})" 
+            using multiset_old_term_insert[of b elem k f X y] elem_group False y_def valid_before disjoint
+            by(simp only: M_def old_M_def group_def old_group_def updated_data_def group_multiset_def Let_def Optimized_Agg.group_def) auto          
+          then have aux: "length(flatten_multiset(insert (meval_trm f elem, y) old_M)) = length(flatten_multiset(old_M - {(meval_trm f elem, y)})) + i" 
+            using both_finite length_flatten_multiset finite_insert i_def len_commute
+            Finite_Set.comp_fun_commute.fold_insert_remove[of "\<lambda>(t, m) y. y + the_enat m" old_M 0 "(meval_trm f elem, y)"] by auto
+          have "(meval_trm f elem, y + 1) \<notin> old_M - {(meval_trm f elem, y)}" using y_def by auto
+          then show ?thesis using len_commute both_finite finite_remove M_insert_remove_def i_def Finite_Set.comp_fun_commute.fold_insert[of "\<lambda>(t, m) y. y + the_enat m" "old_M - {(meval_trm f elem, y)}" "(meval_trm f elem, y + 1)" 0]
+            by (metis (mono_tags, lifting) aux case_prod_conv group_cancel.add1 insert_absorb length_flatten_multiset one_enat_def plus_enat_simps(1) the_enat.simps y_def)
+        qed
+        
+        moreover have "foldl plus y0 (flatten_multiset M) = (foldl plus y0 (flatten_multiset old_M)) + term'"
+        proof(cases "Set.filter (\<lambda>x. meval_trm f x = meval_trm f elem) old_group = {}")
+          case True
+          then have "M = insert (meval_trm f elem, 1) old_M" using multiset_new_term_insert elem_group by(simp add: Let_def)
+          moreover have "(meval_trm f elem, 1) \<notin> old_M" using True by auto
+          moreover have "foldl (+) y0 (flatten_multiset M) = Finite_Set.fold (\<lambda>(t, m). (plus') t ^^ the_enat m) y0 M"
+            using foldl_flatten_multiset foldl_eint_equival M_int y0_int both_finite comm_plus' comp_fun_commute_plus' by(simp)
+          moreover have "foldl (+) y0 (flatten_multiset old_M) = Finite_Set.fold (\<lambda>(t, m). (plus') t ^^ the_enat m) y0 old_M" 
+            using foldl_flatten_multiset foldl_eint_equival M_old_int y0_int both_finite comm_plus' comp_fun_commute_plus' by simp
+          moreover have "(Finite_Set.fold (\<lambda>(t, m). plus' t ^^ the_enat m) y0 old_M) \<in> range EInt" 
+            using finite_set_fold_int  both_finite old_multiset_int y0_int by blast
+          moreover have "meval_trm f elem \<in> range EInt" using calculation(1) multiset_int by blast
+          ultimately show ?thesis
+            using  both_finite plus_plus'_equiv plus'_iter_one_enat plus'_comp_commute type_restr comm_plus'
+              Finite_Set.comp_fun_commute.fold_insert[of "\<lambda>(t, m). (plus') t ^^ the_enat m"] by simp
+        next
+          case False
+          then obtain y where y_def: "(meval_trm f elem, y) \<in> old_M" 
+            by (smt (z3) Collect_empty_eq Set.filter_def image_eqI old_M_def)
+          then obtain i where i_def: "y = enat i" 
+            by (smt (z3) Pair_inject ecard_def finite_filter image_iff old_M_def old_group_def valid_before valid_maggaux.simps)
+          have finite_remove: "finite (old_M - {(meval_trm f elem, y)})" using both_finite finite_Diff  by (auto simp: Set.remove_def)
+          have finite_insert: "finite (insert (meval_trm f elem, y) old_M)" using both_finite by blast
+          have M_insert_remove_def: "M = insert (meval_trm f elem, y + 1) (old_M - {(meval_trm f elem, y)})" 
+            using multiset_old_term_insert[of b elem k f X y] elem_group False y_def valid_before disjoint
+            by(simp only: M_def old_M_def group_def old_group_def updated_data_def group_multiset_def Let_def Optimized_Agg.group_def) auto 
+          have foldl_plus_plus'_equiv: "foldl (+) y0 (flatten_multiset M) = foldl (plus') y0 (flatten_multiset M)" using foldl_eint_equival M_int y0_int by auto
+          have aux1: "foldl (plus') y0 (flatten_multiset (insert (term', y) old_M)) = Finite_Set.fold (\<lambda>(t, m). (plus') t ^^ the_enat m) y0 (insert (term', y) old_M)"
+            using foldl_flatten_multiset[of "insert (term', y) old_M" plus' y0] finite_insert comp_fun_commute_plus' comm_plus' by auto
+          moreover have foldl_remove_equiv: "foldl plus' y0 (flatten_multiset(old_M - {(term', y)})) = Finite_Set.fold (\<lambda>(t, m). (plus') t ^^ the_enat m) y0 (old_M - {(term', y)})"
+            using foldl_flatten_multiset[of "old_M - {(term', y)}" plus' y0] finite_insert comp_fun_commute_plus' comm_plus' by auto
+          ultimately have aux: "foldl plus' y0 (flatten_multiset(insert (term', y) old_M)) = ((plus' term') ^^ (the_enat y)) (foldl plus' y0 (flatten_multiset(old_M - {(term', y)})))" 
+            using  finite_insert plus'_comp_commute Finite_Set.comp_fun_commute.fold_insert_remove[of "\<lambda>(t, m). (plus') t ^^ the_enat m"] by auto
+          moreover have term'_int: "term' \<in> range EInt" using old_multiset_int term'_def y_def by blast
+          moreover have "foldl plus' y0 (flatten_multiset(old_M - {(term', y)})) \<in> range EInt" 
+            using foldl_remove_equiv by (metis DiffD1 finite_remove finite_set_fold_int old_multiset_int term'_def y0_int)
+          ultimately have aux: "foldl plus' y0 (flatten_multiset(old_M - {(term', y)})) = ((minus' term') ^^ (the_enat y)) (foldl plus' y0 (flatten_multiset(old_M)))"
+            using plus'_minus'_id by (metis comp_apply insert_absorb term'_def y_def)
+          moreover have "(term', y + 1) \<notin> old_M - {(term', y)}" using y_def by auto
+          ultimately have "Finite_Set.fold (\<lambda>(t, m). (plus') t ^^ the_enat m) y0 M = ((plus' term') ^^ (i + 1)) (((minus' term') ^^ i) (foldl plus' y0 (flatten_multiset(old_M))))"
+            using Finite_Set.comp_fun_commute.fold_insert[of "\<lambda>(t, m). plus' t ^^ the_enat m"] plus'_comp_commute finite_remove i_def
+            by(simp only: M_insert_remove_def term'_def) (metis (no_types, lifting) case_prod_conv foldl_remove_equiv one_enat_def plus_enat_simps(1) term'_def the_enat.simps)
+          moreover have "foldl (plus') y0 (flatten_multiset(M)) = Finite_Set.fold (\<lambda>(t, m). (plus') t ^^ the_enat m) y0 M"
+            using foldl_flatten_multiset[of M plus' y0] both_finite comp_fun_commute_plus' comm_plus' by auto
+          ultimately have "foldl (plus') y0 (flatten_multiset(M)) = plus' term' (foldl plus' y0 (flatten_multiset(old_M)))"
+            using aux1 by (smt (z3) add.commute aux both_finite comp_eq_dest_lhs comp_fun_commute.fold_insert_remove foldl_remove_equiv funpow_add i_def insert_absorb old.prod.case plus'_comp_commute plus'_iter_one term'_def the_enat.simps y_def)
+          moreover have "foldl plus' y0 (flatten_multiset(old_M)) \<in> range EInt" 
+            by (metis aux1 both_finite finite_set_fold_int insert_absorb old_multiset_int term'_def y0_int y_def)
+          ultimately show ?thesis 
+            using plus_plus'_equiv foldl_plus_plus'_equiv term'_int M_old_int comm_plus' foldl_eint_equival y0_int by auto
+        qed
+        ultimately show ?thesis using len_def sum_def by auto
+      next
+        case False
+        then have same_group: "group = old_group" by auto
+        then have "M = old_M" by auto
+        then have "Mapping.lookup updated_map k = Mapping.lookup m k" 
+          using False by (auto split:option.splits simp:Let_def lookup_update')
+        then show ?thesis using valid_before same_group in_map 
+          by (auto simp: Let_def)
+      qed
+    qed
+  qed
+  have valid_type_restr: "type_restr \<lparr>aggargs_cols = cols, aggargs_n = n, aggargs_g0 = g0, aggargs_y = y, aggargs_\<omega> = \<omega>, aggargs_b = b, aggargs_f = f\<rparr> (insert elem X)"
+    using valid_before type_restr by (auto simp:type_restr_def Let_def)
+  show ?thesis using valid_value_invariant valid_key_invariant valid_finite valid_before valid_type_restr
+    by (auto simp:Let_def)
+qed
 
 lemma valid_insert_cnt_unfolded: 
   assumes valid_before: "valid_maggaux \<lparr>aggargs_cols = cols, aggargs_n = n, aggargs_g0 = g0, aggargs_y = y, aggargs_\<omega> = \<omega>, aggargs_b = b, aggargs_f = f\<rparr> (CntAux m) X" 
   and disjoint: "elem \<notin> X"
-shows "valid_maggaux \<lparr>aggargs_cols = cols, aggargs_n = n, aggargs_g0 = g0, aggargs_y = y, aggargs_\<omega> = \<omega>, aggargs_b = b, aggargs_f = f\<rparr> 
+  shows "valid_maggaux \<lparr>aggargs_cols = cols, aggargs_n = n, aggargs_g0 = g0, aggargs_y = y, aggargs_\<omega> = \<omega>, aggargs_b = b, aggargs_f = f\<rparr> 
         (CntAux (insert_cnt \<lparr>aggargs_cols = cols, aggargs_n = n, aggargs_g0 = g0, aggargs_y = y, aggargs_\<omega> = \<omega>, aggargs_b = b, aggargs_f = f\<rparr> elem m)) (X \<union> {elem})"
 proof - 
   define updated_map where [simp]: "updated_map = insert_cnt \<lparr>aggargs_cols = cols, aggargs_n = n, aggargs_g0 = g0, aggargs_y = y, aggargs_\<omega> = \<omega>, aggargs_b = b, aggargs_f = f\<rparr> elem m"
@@ -417,6 +822,7 @@ lemma valid_insert_maggaux_unfolded:
   "valid_maggaux \<lparr>aggargs_cols = cols, aggargs_n = n, aggargs_g0 = g0, aggargs_y = y, aggargs_\<omega> = \<omega>, aggargs_b = b, aggargs_f = f\<rparr> aux X \<Longrightarrow>
   finite Y \<Longrightarrow>
   X \<inter> Y = {} \<Longrightarrow>
+  type_restr \<lparr>aggargs_cols = cols, aggargs_n = n, aggargs_g0 = g0, aggargs_y = y, aggargs_\<omega> = \<omega>, aggargs_b = b, aggargs_f = f\<rparr> Y \<Longrightarrow>
   valid_maggaux \<lparr>aggargs_cols = cols, aggargs_n = n, aggargs_g0 = g0, aggargs_y = y, aggargs_\<omega> = \<omega>, aggargs_b = b, aggargs_f = f\<rparr> 
   (insert_maggaux \<lparr>aggargs_cols = cols, aggargs_n = n, aggargs_g0 = g0, aggargs_y = y, aggargs_\<omega> = \<omega>, aggargs_b = b, aggargs_f = f\<rparr> Y aux) (X \<union> Y)" 
 proof(induction aux)
@@ -442,15 +848,73 @@ proof(induction aux)
     ultimately have "insert_maggaux args (insert x F) (CntAux m) = CntAux (insert_cnt args x intermediate_map)"
       using  Finite_Set.comp_fun_commute.fold_insert[of "insert_cnt args" F x m]
       by auto
-    then have "valid_maggaux args (insert_maggaux args (insert x F) (aggaux.CntAux m)) (X \<union> insert x F)"
+    then have "valid_maggaux args (insert_maggaux args (insert x F) (CntAux m)) (X \<union> insert x F)"
       using valid_a
       by auto
     then show ?case
       by (auto simp: args_def)
   qed
 next
-case (SumAux x)
-  then show ?case sorry
+  case (SumAux m)
+  have disjoint: "X \<inter> Y = {}" using SumAux by auto
+  have valid_before: "valid_maggaux \<lparr>aggargs_cols = cols, aggargs_n = n, aggargs_g0 = g0, aggargs_y = y, aggargs_\<omega> = \<omega>, aggargs_b = b, aggargs_f = f\<rparr> (SumAux m) X" using SumAux by auto
+  have type_restr: "type_restr \<lparr>aggargs_cols = cols, aggargs_n = n, aggargs_g0 = g0, aggargs_y = y, aggargs_\<omega> = \<omega>, aggargs_b = b, aggargs_f = f\<rparr> Y" using SumAux by auto
+  have finite_y: "finite Y" using SumAux by auto
+  then show ?case using disjoint type_restr valid_before
+  proof(induction Y)
+    case empty
+    then show ?case using SumAux by auto
+  next
+    case (insert x F)
+    define args where "args = \<lparr>aggargs_cols = cols, aggargs_n = n, aggargs_g0 = g0, aggargs_y = y, aggargs_\<omega> = \<omega>, aggargs_b = b, aggargs_f = f\<rparr>"
+    interpret comp_fun_commute "insert_sum_comm args"
+      using insert_sum_comm by unfold_locales auto
+    obtain intermediate_map where intermediate_map_def: "SumAux intermediate_map = insert_maggaux args F (SumAux m)" by auto
+    then have intermediate_map_def': "intermediate_map = Finite_Set.fold (insert_sum args) m F" by auto
+    have "X \<inter> F = {}" using insert(4) by auto
+    moreover have "type_restr args F" using insert(5)  by (cases "fst \<omega>") (auto simp: args_def type_restr_def Let_def) 
+    moreover have "valid_maggaux args (SumAux m) X" using valid_before by (auto simp:args_def)
+    ultimately have valid_int: "valid_maggaux args (SumAux intermediate_map) (X \<union> F)" using insert(3) by(simp only:intermediate_map_def args_def)
+    moreover have "x \<notin> X \<union> F" using insert(2) insert.prems(1) by auto
+    moreover have type_x: "type_restr args {x}" using insert(5) by (cases "fst \<omega>") (auto simp: args_def type_restr_def Let_def) 
+    ultimately have valid_a: "valid_maggaux args (SumAux (insert_sum args x intermediate_map)) (X \<union> F \<union> {x})" 
+      using valid_insert_sum_unfolded[of cols n g0 y \<omega> b f intermediate_map "(X \<union> F)" x] by(auto simp: args_def)
+    have y0_int: "snd (aggargs_\<omega> args) \<in> range EInt" using insert(5) SumAux.prems(1) by (auto simp: type_restr_def args_def Let_def)
+    have aux1: "(\<And>a b. a \<in> (insert x F) \<Longrightarrow> b \<in> valid_sumaux_maps \<Longrightarrow> insert_sum args a b = insert_sum_comm args a b)" 
+    proof -
+      fix a b
+      assume a_def: "a \<in> (insert x F)" and b_def: "b \<in> valid_sumaux_maps"
+      have "meval_trm (aggargs_f args) a \<in> range EInt" using insert(5) a_def SumAux.prems(1) by(auto simp: type_restr_def Let_def args_def split:option.splits) (auto) 
+      then show "insert_sum args a b = insert_sum_comm args a b" using y0_int b_def insert_sum_equiv[of args a b] by auto
+    qed
+    moreover have aux2: "(\<And>a b. a \<in> (insert x F) \<Longrightarrow> b \<in> valid_sumaux_maps \<Longrightarrow> insert_sum_comm args a b \<in> valid_sumaux_maps)"
+    proof -
+      fix a b
+      assume "a \<in> (insert x F)" and "b \<in> valid_sumaux_maps"
+      then show "insert_sum_comm args a b \<in> valid_sumaux_maps"
+        using y0_int 
+        apply(auto simp: valid_sumaux_maps_def  Let_def lookup_update' split:option.splits) 
+        by fastforce fastforce
+    qed
+    moreover have valid_m: "m \<in> valid_sumaux_maps" using valid_maggaux_valid_map SumAux(1) by auto
+    ultimately have "Finite_Set.fold (insert_sum args) m (insert x F) = Finite_Set.fold (insert_sum_comm args) m (insert x F)"
+      using sumaux_finite_set_fold_eq[of "(insert x F)" "insert_sum args" "insert_sum_comm args" m] insert by auto
+    moreover have "Finite_Set.fold (insert_sum args) m F = Finite_Set.fold (insert_sum_comm args) m F"
+      using sumaux_finite_set_fold_eq[of F "insert_sum args" "insert_sum_comm args" m] using insert aux1 aux2 valid_m by auto
+    moreover have "Finite_Set.fold (insert_sum_comm args) m (insert x F) = insert_sum_comm args x (Finite_Set.fold (insert_sum_comm args) m F)"
+      using  Finite_Set.comp_fun_commute.fold_insert[of "insert_sum_comm args" F x m] insert by auto
+    moreover have "Finite_Set.fold (insert_sum args) m F \<in> valid_sumaux_maps" 
+      using valid_maggaux_valid_map[of cols n g0 y \<omega> b f intermediate_map "X \<union> F"] intermediate_map_def' valid_int by(simp only:args_def)
+    moreover have "meval_trm (aggargs_f args) x \<in> range EInt" 
+      using type_x SumAux.prems(1) by(auto simp: type_restr_def Let_def args_def split:option.splits)
+    ultimately have "Finite_Set.fold (insert_sum args) m (insert x F) = insert_sum args x (Finite_Set.fold (insert_sum args) m F)"
+      using insert_sum_equiv[of args x "Finite_Set.fold (insert_sum args) m F"] y0_int by auto
+    then have "insert_maggaux args (insert x F) (SumAux m) = SumAux (insert_sum args x intermediate_map)"
+      using intermediate_map_def' by auto
+    then have "valid_maggaux args (insert_maggaux args (insert x F) (SumAux m)) (X \<union> insert x F)"
+      using valid_a by auto
+    then show ?case by (simp only: args_def)
+  qed
 next
   case (MinAux x)
   then show ?case sorry
